alloc/Mman.fst
@@ -1,8 +1,16 @@
 module Mman
 
+open Steel.Effect.Atomic
+open Steel.Effect
+module A = Steel.Array
+
 module U64 = FStar.UInt64
 module U32 = FStar.UInt32
 module I32 = FStar.Int32
+module U8 = FStar.UInt8
+
+let array = Steel.ST.Array.array
+
 
 noextract
 assume val mmap
@@ -12,7 +20,23 @@ assume val mmap
   (flags: I32.t)
   (fildes: I32.t)
   (off: U32.t)
-  : U64.t
+  : Steel (array U8.t)
+    emp
+    (fun a -> A.varray a)
+    (fun _ -> True)
+    (fun _ a h1 ->
+      A.length a == U64.v len /\
+      A.is_full_array a /\
+      A.asel a h1 == Seq.create (U64.v len) U8.zero
+    )
 
 noextract
-assume val munmap (addr: U64.t) (size_t: U64.t): U32.t
+assume val munmap (a: array U8.t) (size_t: U64.t)
+  : Steel unit
+    (A.varray a)
+    (fun _ -> emp)
+    (fun _ ->
+      A.length a == U64.v size_t /\
+      A.is_full_array a
+    )
+    (fun _ _ _ -> True)
